% Created 2019-09-13 äº” 18:25
% Intended LaTeX compiler: pdflatex
\documentclass[11pt]{article}
\usepackage[utf8]{inputenc}
\usepackage[T1]{fontenc}
\usepackage{graphicx}
\usepackage{grffile}
\usepackage{longtable}
\usepackage{wrapfig}
\usepackage{rotating}
\usepackage[normalem]{ulem}
\usepackage{amsmath}
\usepackage{textcomp}
\usepackage{amssymb}
\usepackage{capt-of}
\usepackage{hyperref}
\usepackage{minted}
\input{preamble.tex}
\author{Joseph J. Rotman}
\date{\today}
\title{Advanced Modern Algebra}
\hypersetup{
 pdfauthor={Joseph J. Rotman},
 pdftitle={Advanced Modern Algebra},
 pdfkeywords={},
 pdfsubject={},
 pdfcreator={Emacs 26.2 (Org mode 9.2.5)}, 
 pdflang={English}}
\begin{document}

\maketitle
\tableofcontents \clearpage
\section{Group \rom{1}}
\label{sec:orgb5b47d9}
\subsection{Permutations}
\label{sec:orgb90d65f}
\begin{definition}[]
A \textbf{permutation} of a set \(X\) is a bijection from \(X\) to itself.
\end{definition}


\begin{definition}[]
The family of all the permutations of a set \(X\), denoted by \(S_X\) is called
the \textbf{symmetric group} on \(X\). When \(X=\lb 1,2,\dots,n\rb\), \(S_X\) is
usually denoted by \(X_n\) and is called the \textbf{symmetric group on } \(n\)
\textbf{letters} 
\end{definition}

\begin{definition}[]
Let \(i_1,i_2,\dots,i_r\) be distinct integers in \(\lb 1,2,\dots,n\rb\). If
\(\alpha\in S_n\) fixes the other integers and if
\begin{equation*}
\alpha(i_1)=i_2,\alpha(i_2)=i_3,\dots,\alpha(i_{r-1})=i_r,\alpha(i_r)=i_1
\end{equation*}
then \(\alpha\) is called an textbf\{r-cycle\}. \(\alpha\) is a cycle of
\textbf{length} \(r\) and denoted by
\begin{equation*}
\alpha=(i_1\; i_2\;\dots\; i_r)
\end{equation*}
\end{definition}

2-cycles are also called the \textbf{transpositions}.

\begin{definition}[]
Two permutations \(\alpha,\beta\in S_n\) are \textbf{disjoint} if every \(i\)
moved by one is fixed by the other.
\end{definition}

\begin{lemma}[]
Disjoint permutations \(\alpha,\beta\in S_n\) commute
\end{lemma}

\begin{proposition}[]
Every permutation \(\alpha\in S_n\) is either a cycle or a product of disjoint cycles.
\end{proposition}

\begin{proof}
Induction on the number \(k\) of points moved by \(\alpha\)
\end{proof}

\begin{definition}[]
A \textbf{complete factorization} of a permutation \(\alpha\) is a
factorization of \(\alpha\) into disjoint cycles that contains exactly one
1-cycle \((i)\) for every \(i\) fixed by \(\alpha\)
\end{definition}

\begin{theorem}[]
Let \(\alpha\in S_n\) and let \(\alpha=\beta_1\dots\beta_t\) be a complete
factorization into disjoint cycles. This factorization is unique except for
the order in which the cycles occur
\end{theorem}

\begin{proof}
for all \(i\), if \(\beta_t(i)\neq i\), then \(\beta_t^k(i)\neq\beta_t^{k-1}(i)\)
for any \(k\ge 1\)
\end{proof}

\begin{lemma}[]
If \(\gamma,\alpha\in S_n\), then \(\alpha\gamma\alpha^{-1}\) has the same cycle
structure as \(\gamma\). In more detail, if the complete factorization of
\(\gamma\) is
\begin{equation*}
\gamma=\beta_1\beta_2\dots(i_1\; i_2\;\dots)\dots\beta_t
\end{equation*}
then \(\alpha\gamma\alpha^{-1}\) is permutation that is obtained from \(\gamma\)
by applying \(\alpha\) to the symbols in the cycles of \(\gamma\)
\end{lemma}

Example. Suppose
\begin{gather*}
\beta=(1\;2\;3)(4)(5)\\
\gamma=(5\;2\;4)(1)(3)
\end{gather*}
then we can easily find the \(\alpha\)
\begin{equation*}
\alpha=
\begin{pmatrix}
1&2&3&4&5\\
5&2&4&1&3
\end{pmatrix}
\end{equation*}
\begin{theorem}[]
Permutations \(\gamma\) and \(\sigma\) in \(S_n\) has the same cycle structure if
and only if there exists \(\alpha\in S_n\) with \(\sigma=\alpha\gamma\alpha^{-1}\)
\end{theorem}


\begin{proposition}[]
If \(n\ge 2\) then every \(\alpha\in S_n\) is a product of tranpositions
\end{proposition}
\begin{proof}
\((1\;2\;\dots\; r)=(1\; r)(1\; r-1)\dots(1\; 2)\)
\end{proof}


\begin{definition}[]
A permutation \(\alpha\in S_n\) is \textbf{even} if it can be factored into a
product of an even number of transpositions. Otherwise \textbf{odd}
\end{definition}

\begin{definition}[]
If \(\alpha\in S_n\) and \(\alpha=\beta_1\dots\beta_t\) is a complete
factorization, then \textbf{signum} \(\alpha\) is defined by
\begin{equation*}
\sgn(\alpha)=(-1)^{n-t}
\end{equation*}
\end{definition}

\begin{theorem}[]
For all \(\alpha,\beta\in S_n\)
\begin{equation*}
\sgn(\alpha\beta)=\sgn(\alpha)\sgn(\beta)
\end{equation*}
\end{theorem}

\begin{theorem}[]
\begin{enumerate}
\item Let \(\alpha\in S_n\); if \(\sgn(\alpha)=1\) then \(\alpha\) is even. otherwise
odd
\item A permutation \(\alpha\) is odd if and only if it's a product of an odd
number of transpositions
\end{enumerate}
\end{theorem}

\begin{corollary}[]
Let \(\alpha,\beta\in S_n\). If \(\alpha\) and \(\beta\) have the same parity, then
\(\alpha\beta\) is even while if \(\alpha\) and \(\beta\) have distinct parity,
\(\alpha\beta\) is odd
\end{corollary}
\subsection{Groups}
\label{sec:org0a25b16}
\begin{definition}[]
A \textbf{binary operation} on a set \(G\) is a function
\begin{equation*}
*:G\times G\to G
\end{equation*}
\end{definition}

\begin{definition}[]
A \textbf{group} is a set \(G\) equipped with a binary operation * s.t.
\begin{enumerate}
\item the \textbf{associative law} holds
\item \textbf{identity}
\item every \(x\in G\) has an \textbf{inverse}, there is a \(x'\in G\)  with 
\(x*x'=e=x'*x\)
\end{enumerate}
\end{definition}

\begin{definition}[]
A group \(G\) is called \textbf{abelian} if it satisfies the
\textbf{commutative law}
\end{definition}

\begin{lemma}[]
Let \(G\) be a group
\begin{enumerate}
\item The \textbf{cancellation laws} holds: if either \(x*a=x*b\) or \(a*x=b*x\), then
\(a=b\)
\item \(e\) is unique
\item Each \(x\in G\) has a unique inverse
\item \((x^{-1})^{-1}=x\)
\end{enumerate}
\end{lemma}

\begin{definition}[]
An expression \(a_1a_2\dots a_n\) \textbf{needs no parentheses} if all the ultimate
products it yields are equal
\end{definition}

\begin{theorem}[Generalized Associativity]
If \(G\) is a group and \(a_1,a_2,\dots,a_n\in G\) then the expression
\(a_1a_2\dots a_n\) needs no parentheses
\end{theorem}

\begin{definition}[]
Let \(G\) be a group and let \(a\in G\). If \(a^k=1\) for some \(k>1\) then the
smallest such exponent \(k\ge 1\) is called the \tf{order} or \(a\); if no such
power exists, then one says that \(a\) has \tf{infinite order}
\end{definition}

\begin{proposition}[]
If \(G\) is a finite group, then every \(x\in G\) has finite order
\end{proposition}

\begin{definition}[]
A \tf{motion} is a distance preserving bijection \(\varphi:\R^2\to\R^2\). If
\(\pi\) is a polygon in the plane, then its \tf{symmetry group} \(\Sigma(\pi)\)
consists of all the motions \(\varphi\) for which \(\varphi(\pi)=\pi\). The
elements of \(\Sigma(\pi)\) are called the \tf{symmetries} of \(\pi\)
\end{definition}

Let \(\pi_4\) be a square. Then the group \(\Sigma(\pi_4)\) is called the
\tf{dihedral group} with 8 elements, denoted by \(D_8\)

\begin{definition}[]
If \(\pi_n\) is a regular polygon with \(n\) vertices \(v_1,\dots,v_n\) and center
\(O\), then the symmetry group \(\Sigma(\pi_n)\) is called the \tf\{dihedral
group\} with \(2n\) elements, and it's denoted by \(D_{2n}\)
\end{definition}
\subsection{Lagrange's theorem}
\label{sec:org092818e}
\begin{definition}[]
A subset \(H\) of a group \(G\) is a \tf{subgroup} if
\begin{enumerate}
\item \(1\in H\)
\item if \(x,y\in H\), then \(xy\in H\)
\item if \(x\in H\), then \(x^{-1}\in H\)
\end{enumerate}
\end{definition}

If \(H\) is a subgroup of \(G\), we write \(H\le G\). If \(H\) is a proper subgroup,
then we write \$H<\$G

\begin{proposition}[]
A subset \(H\) of a group \(G\) is a subgroup if and only if \(H\) is nonempty and
whenever \(x,y\in H\), \(xy^{-1}\in H\)
\end{proposition}

\begin{proposition}[]
A nonempty subset \(H\) of a finite group \(G\) is a subgroup if and only if \(H\)
is closed; that is, if \(a,b\in H\), then \(ab\in H\)
\end{proposition}

\begin{definition}[]
If \(G\) is a group and \(a\in G\)
\begin{equation*}
\langle a\rangle=\{a^n:n\in\Z\}=\{\text{all powers of } a\}
\end{equation*}
\(\la a\ra\) is called the \tf{cyclic subgroup} of \(G\) \tf{generated} by \(a\). A
group \(G\) is called \tf{cyclic} if there exists \(a\in G\) s.t. \(G=\la a\ra\),
in which case \(a\) is called the \tf{generator}
\end{definition}

\begin{definition}[]
The \tf{integers mod $m$}, denoted by \(\I_m\) is the family of all congruence
classes mod \(m\)
\end{definition}


\begin{proposition}[]
Let \(m\ge 2\) be a fixed integer
\begin{enumerate}
\item If \(a\in \Z\), then \([a]=[r]\) for some \(r\) with \(0\le r<m\)
\item If \(0\le r'<r<m\), then \([r']\neq[r]\)
\item \(\I_m\) has exactly \(m\) elements
\end{enumerate}
\end{proposition}

\begin{theorem}[]
\begin{enumerate}
\item If \(G=\la a\ra\) is a cyclic group of order \(n\), then \(a^k\) is a generator
of \(G\) if and only if \((k,n)=1\)
\item If \(G\) is a cyclic group of order \(n\) and \(\gen(G)=\{\text{all generators
      of } G\}\), then
\begin{equation*}
\abs{\gen(G)}=\phi(n)
\end{equation*}
where \(\phi\) is the Euler \(\phi\)-function
\end{enumerate}
\end{theorem}
\begin{proof}
\begin{enumerate}
\item there is \(t\in\N\) s.t. \(a^{kt}=a\) hence \(a^{kt-1}=1\) and \(n\mid kt-1\)
\end{enumerate}
\end{proof}

\begin{proposition}[]
Let \(G\) be a finite group and let \(a\in G\). Then the order of \(a\) is
\(\abs{\la a\ra}\).
\end{proposition}

\begin{definition}[]
If \(G\) is a finite group, then the number of elements in \(G\), denoted by
\(\abs{G}\) is called the \tf{order} of \(G\)
\end{definition}


\begin{proposition}[]
The intersection \(\bigcap_{i\in I}H_i\) of any family of subgroups of a group
\(G\) is again a subgroup of \(G\)
\end{proposition}


\begin{corollary}[]
If \(X\) is a subset of a group \(G\), then there is a subgroup \(\la X\ra\) of \(G\)
containing \(X\) tHhat is \tf{smallest} in the sense that \(\la X\ra\le H\) for
every subgroup \(H\) 
of \(G\) that contains \(X\)
\end{corollary}


\begin{definition}[]
If \(X\) is a subset of a group \(G\), then \(\la X\ra\) is called the \tf\{subgroup
generated by\} \(X\)
\end{definition}

A \tf{word} on \(X\) is an element \(g\in G\) of the form \(g=x_1^{e_1}\dots
   x_n^{e_n}\) where \(x_i\in X\) and \(e_i=\pm 1\) for all \(i\)

\begin{proposition}[]
If \(X\) is a nonempty subset of a group \(G\), then \(\la X\ra\) is the set of all
words on \(X\)
\end{proposition}


\begin{definition}[]
If \(H\le G\) and \(a\in G\), then the \tf{coset} \(aH\) is the subset \(aH\) of \(G\),
where
\begin{equation*}
aH=\{ah:h\in H\}
\end{equation*}
\end{definition}
\(aH\) \tf{left coset}, \(Ha\) \tf{right coset}

\begin{lemma}[]
\(H\le G,a,b\in G\)
\begin{enumerate}
\item \(aH=bH\) if and only if \(b^{-1}a\in H\)
\item if \(aH\cap bH\neq\emptyset\), then \(aH=bH\)
\item \(\abs{aH}=\abs{H}\) for all \(a\in G\)
\end{enumerate}
\end{lemma}
\begin{proof}
define a relation \(a\equiv b\) if \(b^{-1}a\in H\)
\end{proof}


\begin{theorem}[Lagrange's Theorem]
If \(H\) is a subgroup of a finite group \(G\), then \(\abs{H}\) is a divisor of \(\abs{G}\)
\end{theorem}

\begin{proof}
Let \(\{a_1H,a_2H,\dots,a_tH\}\) be the family of all the distinct cosets of
\(H\) in \(G\). Then
\begin{equation*}
G=a_1H\cup a_2H\cup\dots\cup a_tH
\end{equation*}
hence
\begin{equation*}
\abs{G}=\abs{a_1H}+\dots+\abs{a_tH}
\end{equation*}
But \(\abs{a_iH}=\abs{H}\) for all \(i\). Hence \(\abs{G}=t\abs{H}\)
\end{proof}

\begin{definition}[]
The \tf{index} of a subgroup \(H\) in \(G\) denoted by \([G:H]\), is the number of
left cosets of \(H\) in \(G\)
\end{definition}

Note that \(\abs{G}=[G:H]\abs{H}\)

\begin{corollary}[]
If \(G\) is a finite group and \(a\in G\), then the order of \(a\) is a divisor of
\(\abs{G}\) 
\end{corollary}

\begin{corollary}[]
If \(G\) is a finite group, then \(a^{\abs{G}}=1\) for all \(a\in G\)
\end{corollary}

\begin{corollary}[]
If \(p\) is a prime, then every group \(G\) of order \(p\) is cyclic
\end{corollary}

\begin{proposition}[]
The set \(U(\I_m)\), defined by
\begin{equation*}
 U(\I_m)=\{[r]\in\I_m:(r,m)=1\}
\end{equation*}
is a multiplicative group of order \(\varphi(m)\). If \(p\) is a prime, then
\(U(\I_m)=\I_m^{\times}\), the nonzero elements of \(\I_p\).
\end{proposition}

\begin{corollary}[Fermat]
If \(p\) is a prime and \(a\in\Z\), then
\begin{equation*}
a^p\equiv a\mod p
\end{equation*}
\end{corollary}

\begin{proof}
suffices to show \([a^p]=[a]\) in \(\I_p\). If \([a]=[0]\), then \([a^p]=[a]^p=[0]\).
Else, since \(\abs{\I_p^\times}=p-1\), \([a]^{p-1}=[1]\)
\end{proof}


\begin{theorem}[Euler]
If \((r,m)=1\), then
\begin{equation*}
r^{\phi(m)}\equiv 1\mod m
\end{equation*}
\end{theorem}

\begin{theorem}[Wilson's Theorem]
An integer \(p\) is a prime if and only if
\begin{equation*}
(p-1)!\equiv -1\mod p
\end{equation*}
\end{theorem}
\subsection{Homomorphisms}
\label{sec:org955d913}
\begin{definition}[]
If \((G,*)\) and \((H,\circ)\) are groups, then a function \(f:G\to H\) is a
\tf{homomorphism} if
\begin{equation*}
f(x*y)=f(x)\circ f(y)
\end{equation*}
for all \(x,y\in G\). If \(f\) is also a bijection, then \(f\) is called an
\tf{isomorphism}. \(G\) and \(H\) are called \tf{isomorphic}, denoted by \(G\cong H\)
\end{definition}

\begin{lemma}[]
Let \(f:G\to H\) be a homomorphism
\begin{enumerate}
\item \(f(1)=1\)
\item \(f(x^{-1})=f(x)^{-1}\)
\item \(f(x^n)=f(x)^n\) for all \(n\in\Z\)
\end{enumerate}
\end{lemma}

\begin{definition}[]
If \(f:G\to H\) is a homomorphism, define
\begin{equation*}
\tf{kernel}f=\{x\in G:f(x)=1\}
\end{equation*}
and
\begin{equation*}
\tf{image}f=\{h\in H:h=f(x)\text{ for some } x\in G\}
\end{equation*}
\end{definition}

\begin{proposition}[]
Let \(f:G\to H\) be a homomorphism
\begin{enumerate}
\item \(\ker f\) is a subgroup of \(G\) and \(\im f\) is a subgroup of \(H\)
\item if \(x\in\ker f\) and if \(a\in G\), then \(axa^{-1}\in\ker f\)
\item \(f\) is an injection if and only if \(\ker f=\{1\}\)
\end{enumerate}
\end{proposition}

\begin{proof}
\begin{enumerate}
\item \(f(a)=f(b)\Leftrightarrow f(ab^{-1})=1\)
\end{enumerate}
\end{proof}

\begin{definition}[]
A subgroup \(K\) of a group \(G\) is called a \tf{normal subgroup} if \(k\in K\)
and \(g\in G\) imply \(gkg^{-1}\in K\), denoted by \(K\triangleleft G\)
\end{definition}

\begin{definition}[]
If \(G\) is a group and \(a\in G\), then a \tf{conjugate} of \(a\) is any element
in \(G\) of the form
\begin{equation*}
gag^{-1}
\end{equation*}
where \(g\in G\)
\end{definition}

\begin{definition}[]
If \(G\) is a group and \(g\in G\), define \tf{conjugation} \(\gamma_g:G\to G\) by
\begin{equation*}
\gamma_g(a)=gag^{-1}
\end{equation*}
for all \(a\in G\)
\end{definition}

\begin{proposition}[]
\begin{enumerate}
\item If \(G\) is a group and \(g\in G\), then conjugation \(\gamma_g:G\to G\) is an
isomorphism
\item Conjugate elements have the same order
\end{enumerate}
\end{proposition}

\begin{proof}
\begin{enumerate}
\item bijection: \(\gamma_g\circ\gamma_{g^{-1}}=1=\gamma_{g^{-1}}\circ\gamma_g\)
\end{enumerate}
\end{proof}

\begin{proposition}[]
\begin{enumerate}
\item If \(H\) is a subgroup of index 2 in a group \(G\), then \(g^2\in H\) for every
\(g\in G\)
\item If \(H\) is a subgroup of index 2 in a group \(G\), then \(H\) is a normal
subgroup of \(G\)
\end{enumerate}
\end{proposition}

\begin{definition}[]
The group of \tf{quaternions} is the group \(\bQ\) of order 8 consisting of the
following matrices in \(GL(2, \C)\)
\begin{equation*}
\bQ=\{I,A,A^2,A^3,B,BA,BA^2,BA^3\}
\end{equation*}
where \(I\) is the identity matrix
\begin{equation*}
A=
\begin{pmatrix}
0&1\\
-1&0
\end{pmatrix}, \text{ and }
B=\begin{pmatrix}
0&i\\
i&0
  \end{pmatrix}
\end{equation*}
\end{definition}


\begin{proposition}[]
The alternating group \(A_4\) is a group of order 12 having no subgroup of
order 6
\end{proposition}
\subsection{Quotient group}
\label{sec:org256de84}
\(\cals(G)\) is the set of all nonempty subsets of a group \(G\). If
\(X,Y\in\cals(G)\), define
\begin{equation*}
XY=\{xy:x\in X\text{ and } y\in Y\}
\end{equation*}

\begin{lemma}[]
\(K\le G\) is normal if and only if
\begin{equation*}
gK=Kg
\end{equation*}
\end{lemma}

A natural question is that whether \(HK\) is a subgroup when \(H\) and \(K\) are
subgroups. The answer is no. Let \(G=S_3,H=\la(1\;2)\ra,K=\la(1\;3)\ra\)


\begin{proposition}[]
\begin{enumerate}
\item If \(H\) and \(K\) are subgroups of a group \(G\), and if one of them is normal,
then \(HK\le G\) and \(HK=KH\)
\item If \(H,K\tril G\), then \(HK\tril G\)
\end{enumerate}
\end{proposition}

\begin{theorem}[]
Let \(G/K\) denote the family of all the left cosets of a subgroup \(K\) of \(G\).
If \(K\tril G\), then
\begin{equation*}
aKbK=abK
\end{equation*}
for all \(a,b\in G\) and \(G/K\) is a group under this operation
\end{theorem}

\begin{proof}
\(aKbK=abKK=abK\)
\end{proof}

\(G/K\) is called the \tf{quotient group} \(G\) mod \(K\)

\begin{corollary}[]
Every \(K\tril G\) is the kernel of some homomorphism
\end{corollary}

\begin{proof}
Define the \tf{natural map} \(\pi:G\to G/K\), \(a\mapsto aK\)
\end{proof}

\begin{theorem}[First Isomorphism Theorem]
If \(f:G\to H\) is a homomorphism, then
\begin{equation*}
\ker f\tril G\quad\text{ and }\quad G/\ker f\cong\im f
\end{equation*}
If \(\ker f=K\) and \(\varphi:G/K\to\im f\le H,aK\mapsto f(a)\), then \(\varphi\)
is an isomorphism
\end{theorem}

\tf{Remark}\quad
\begin{tikzcd}
G \arrow[rr,"f"] \arrow[dr,"\pi"]& &
H\\ 
&G/K \arrow[ur,"\varphi"]&
\end{tikzcd}

\begin{proposition}[Product Formula]
If \(H\) and \(K\) are subgroups of a finite group \(G\), then
\begin{equation*}
\abs{HK}\abs{H\cap K}=\abs{H}\abs{K}
\end{equation*}
\end{proposition}

\begin{proof}
Define a function \(f:H\times K\to HK,(h,k)\mapsto hk\). Show that
\(\abs{f^{-1}(x)}=\abs{H\cap K}\). 

Claim that if \(x=hk\), then
\begin{equation*}
f^{-1}(x)=\{(hd,d^{-1}k):d\in H\cap K\}
\end{equation*}
\end{proof}

\begin{theorem}[Second Isomorphism Theorem]
If \(H\tril G, K\le G\), then \(HK\le G,H\cap K\tril G\) and
\begin{equation*}
K/(H\cap K)\cong HK/H
\end{equation*}
\end{theorem}

\begin{proof}
\(hkH=kk^{-1}hkH=kh'H=kH\)
\end{proof}

\begin{theorem}[Third Isomorphism Theorem]
If \(H,K\tril G\) with \(K\le H\), then \(H/K\tril G/K\) and
\begin{equation*}
(G/K)/(H/K)\cong G/H
\end{equation*}
\end{theorem}

\begin{theorem}[Correspondence Theorem]
If \(K\tril G, \pi:G\to G/K\) is the natural map, then
\begin{equation*}
S\mapsto \pi(S)=S/K
\end{equation*}
is a bijection between \(Sub(G;K)\), the family of all those subgroups \(S\) of
\(G\) that contain \(K\), and \(Sub(G/K)\), the family of all the subgroups of
\(G/K\). If we denote \(S/K\) by \(S^*\), then
\begin{enumerate}
\item \(T\le S\le G\) if and only if \(T^*\le S^*\), in which case \([S:T]=[S^*:T^*]\)
\item \(T\tril S\) if and only if \(T^*\tril S^*\), in which case \(S/T\cong S^*/T^*\)
\end{enumerate}
\end{theorem}

\begin{center}
\begin{tikzcd}
G \arrow[d,dash] \arrow[rd]&\\
S \arrow[d,dash] \arrow[rd] & G/K \arrow[d,dash]\\
T \arrow[d,dash] \arrow[rd] & S/K=S^* \arrow[d,dash]\\
K  \arrow[rd] & T/K=T^* \arrow[d,dash]\\
& \{1\}
\end{tikzcd}
\end{center}
\end{document}