% Created 2020-05-07 å›› 11:13
% Intended LaTeX compiler: pdflatex
\documentclass[11pt]{article}
\usepackage[utf8]{inputenc}
\usepackage[T1]{fontenc}
\usepackage{graphicx}
\usepackage{grffile}
\usepackage{longtable}
\usepackage{wrapfig}
\usepackage{rotating}
\usepackage[normalem]{ulem}
\usepackage{amsmath}
\usepackage{textcomp}
\usepackage{amssymb}
\usepackage{capt-of}
\usepackage{imakeidx}
\usepackage{hyperref}
\usepackage{minted}
\input{preamble.tex}
\author{Stanley Burris \& H. P. Sankappanavar}
\date{\today}
\title{A Course In Universal Algebra}
\hypersetup{
 pdfauthor={Stanley Burris \& H. P. Sankappanavar},
 pdftitle={A Course In Universal Algebra},
 pdfkeywords={},
 pdfsubject={},
 pdfcreator={Emacs 26.3 (Org mode 9.3.6)}, 
 pdflang={English}}
\begin{document}

\maketitle \clearpage
\tableofcontents \clearpage
\section{Lattices}
\label{sec:org3a5e393}

\subsection{Definitions of Lattices}
\label{sec:org54ae7ae}
\begin{definition}[]
A nonempty set \(L\) together with two binary operations \(\vee\) and \(\wedge\)
(read "join" and "meet" respectively) on \(L\) is called a \textbf{lattice} if it
satisfies the following identities
\begin{itemize}%[leftmargin=6em]
 \item[L1:] (a) $x\vee y\approx y\vee x$ \par
 (b) $x\wedge y\approx y\wedge x$\hspace*{\fill}(commutative laws)
 \item[L2:] (a) $x\vee(y\vee z)\approx(x\vee y)\vee z$ \par 
 (b) $x\wedge(y\wedge z)\approx(x\wedge y)\wedge z$
 \hspace*{\fill}(associate laws)
 \item[L3:] (a) \(x\vee x\approx x\)\par 
 (b) \(x\wedge x\approx x\)
 \hspace*{\fill}(idempotent laws)
 \item[L4:] (a) \(x\approx x\vee(x\wedge y)\)\par 
 (b) \(x\approx x\wedge(x\vee y)\)
 \hspace*{\fill}(absorption laws)
\end{itemize}
\end{definition}

\begin{definition}[]
Let \(A\) be a subset of a poset \(P\). An element \(p\) in \(P\) is an \textbf{upper bound}
for \(A\) if \(a\le p\) for every \(a\) in \(A\). An element \(p\) in \(P\) is the
\textbf{least upper bound} of \(A\) (l.u.b. of \(A\)) or \textbf{supremum} of \(A\) (\(\sup A\).

For \(a,b\) in \(P\) we say \(b\) \textbf{covers} \(a\), or \(a\) is \textbf{covered by} \(b\) if
\(a<b\) and whenever \(a\le c\le b\) it follows that \(a=c\) or \(c=b\). We
use the notation \(a\prec b\) to denote \(a\) is covered by \(b\). 
\end{definition}

\begin{definition}[]
A poset \(L\) is a lattice iff for every \(a,b\) in \(L\) both \(\sup\{a,b\}\)
and \(\inf\{a,b\}\) exist
\end{definition}

\begin{enumerate}
\item If \(L\) is a lattice by the first definition, then define \(\le\) on \(L\)
by \(a\le b\) iff \(a=a\wedge b\)
\item If \(L\) is a lattice by the second definition, then define \(\vee\) and
\(\wedge\) by \(a\vee b=\sup\{a,b\}\) and \(a\wedge b=\inf\{a,b\}\)
\end{enumerate}


\subsection{Isomorphism Lattices, and Sublattices}
\label{sec:org1eadfc8}
\begin{definition}[]
Two lattices \(L_1\) and \(L_2\) are \textbf{isomorphic} if there is a bijection
\(\alpha\) from \(L_1\) to \(L_2\) s.t. for every \(a,b\) in \(L_1\) the following two
equation hold: \(\alpha(a\vee b)=\alpha(a)\vee\alpha(b)\) and 
\(\alpha(a\wedge b)=\alpha(a)\wedge\alpha(b)\). Such an \(\alpha\) is called an \textbf{isomorphism}
\end{definition}

\begin{definition}[]
If \(P_1\) and \(P_2\) are two posets and \(\alpha\) is a map from \(P_1\) to \(P_2\), then we
say \(\alpha\) is \textbf{order-preserving} if \(\alpha(a)\le\alpha(b)\) holds in \(P_2\) whenever
\(a\le b\) holds in \(P_1\)
\end{definition}

\begin{theorem}[]
Two lattices \(L_1\) and \(L_2\) are isomorphic iff there is a bijection \(\alpha\) from
\(L_1\) to \(L_2\) s.t. both \(\alpha\) and \(\alpha^{-1}\) are order-preserving
\end{theorem}

\begin{definition}[]
If \(L\) is a lattice and \(L'\neq\emptyset\) is a subset of \(L\) s.t. for every
pair of elements \(a,b\) in \(L'\) both \(a\vee b\) and \(a\wedge b\) are in
\(L'\), where \(\wedge,\vee\) are the lattice operations of \(L\), then we say
that \(L'\) with the same operations is a \textbf{sublattice} of \(L\)
\end{definition}

\begin{definition}[]
A lattice \(L_1\) can be \textbf{embedded} into a lattice \(L_2\) if there is a sublattice
of \(L_2\) isomorphic to \(L_1\); in this case we also say that \(L_2\) 
\textbf{contains a copy of \(L_1\) as a sublattice}
\end{definition}

\subsection{Distributive and Modular Lattices}
\label{sec:org162995c}
\begin{definition}[]
A \textbf{distributive lattice} is a lattice which satisfies either  of the
distributive laws,
\begin{itemize}
\item[D1:] \(x\wedge(y\vee z)\approx(x\wedge y)\vee(x\wedge z)\)
\item[D2:] \(x\vee(y\wedge z)\approx(x\vee y)\wedge(x\vee z)\)
\end{itemize}
\end{definition}

\begin{theorem}[]
A lattice \(L\) satisfies D1 iff it satisfies D2
\begin{align*}
x\vee(y\wedge z)&\approx(x\vee(x\wedge z))\vee(y\wedge z)\tag*{(by L4(a))}\\
&\approx x\vee((x\wedge z)\vee(y\wedge z))\\
&\approx x\vee((z\wedge x)\vee(z\wedge y))\\
&\approx x\vee(z\wedge(x\vee y))\\
&\approx x\vee((x\vee y)\wedge z)\\
&\approx (x\wedge(x\vee y))\vee(x\vee y\wedge z)\\
&\approx ((x\vee y)\wedge x)\vee((x\vee y)\wedge)\\
&\approx (x\vee y)\wedge(x\vee z)
\end{align*}
\end{theorem}

Actually every lattice satisfies both of the inequalities
\((x\wedge y)\vee(x\wedge z)\le x\wedge(y\vee z)\) and
\(x\vee(y\wedge z)\le(x\vee y)\wedge(x\vee z)\).

\begin{definition}[]
A \textbf{modular lattice} is any lattice which satisfies the \textbf{modular} law
\begin{itemize}
\item[M:] \(x\le y\to x\vee(y\wedge z)\approx y\wedge(x\vee z)\)
\end{itemize}
\end{definition}
Equivalent to the identity
\begin{equation*}
(x\wedge y)\vee(y\wedge z)\approx y\wedge((x\wedge y)\vee z)
\end{equation*}
Every lattice satisfies
\begin{equation*}
x\le y\to x\vee(y\wedge z)\le y\wedge(x\vee z)
\end{equation*}

\begin{theorem}[]
Every distributive lattice is a modular lattice
\end{theorem}

Neither \(M_5\) nor \(N_5\) is a distributive lattice in Figure \ref{fig:mn}

\begin{figure}[H]
\centering
\begin{subfigure}[b]{0.3\textwidth}
\begin{tikzpicture}
[dot/.style={circle,draw,minimum width=4pt,inner sep=1pt}]
\node[dot,label=left:$a$] (a) at (0,0) {};
\node[dot,label=right:$b$] (b) at (1,0) {};
\node[dot,label=right:$c$] (c) at (2,0) {};
\node[dot] (d) at (1,-1) {};
\node[dot] (e) at (1,1) {};
\path[] (e) edge (a) edge (b) edge (c)
(d) edge (a) edge (b) edge (c);
\end{tikzpicture}
\caption*{$M_5$}
\end{subfigure}
\begin{subfigure}[b]{0.3\textwidth}
\begin{tikzpicture}
[dot/.style={circle,draw,minimum width=4pt,inner sep=1pt}]
\node[dot,label=left:$a$] (a) at (0,-0.5) {};
\node[dot,label=left:$b$] (b) at (0,0.5) {};
\node[dot,label=right:$c$] (c) at (1.5,0) {};
\node[dot] (d) at (1,1) {};
\node[dot] (e) at (1,-1) {};
\path (d) edge (b) edge (c)
(b) edge (a) 
(e) edge (a) edge (c);
\end{tikzpicture}
\caption*{$N_5$}
\end{subfigure}
\caption{}
\label{fig:mn}
\end{figure}

\begin{theorem}[Dedekind]
\label{thm3.5}
\(L\) is a nonmodular lattice iff \(N_5\) can be embedded into \(L\)
\end{theorem}

\begin{proof}
If \(L\) doesn't satisfy the modular law. Then for some \(a,b,c\) in \(L\) we
have \(a\le b\) but \(a\vee(b\wedge c)<b\wedge(a\vee c)\). Let
\(a_1=a\vee(b\wedge c)\) and \(b_1=b\wedge(a\vee c)\). Then
\begin{equation*}
c\wedge b_1=c\wedge(b\wedge(a\vee c))=(c\wedge(a\vee c))\wedge b=c\wedge b
\end{equation*}
and
\begin{equation*}
c\vee a_1=c\vee a
\end{equation*}
Now as \(c\wedge b\le a_1\le b_1\), we have \(c\wedge b\le c\wedge a_1\le
   c\wedge b_1=c\wedge b\), hence \(c\wedge a_1=c\wedge b\). Likewise
\(c\vee a=c\vee b_1\)
\begin{figure}[H]
\centering
\begin{tikzpicture}
[dot/.style={circle,draw,minimum width=4pt,inner sep=1pt}]
\node[dot,label=left:$a_1$] (a) at (0,-0.5) {};
\node[dot,label=left:$b_1$] (b) at (0,0.5) {};
\node[dot,label=right:$c$] (c) at (1.5,0) {};
\node[dot,label=above:$c\vee a$] (d) at (1,1) {};
\node[dot,label=below:$c\wedge b$] (e) at (1,-1) {};
\path (d) edge (b) edge (c)
(b) edge (a) 
(e) edge (a) edge (c);
\end{tikzpicture}
\caption{}
\end{figure}
\end{proof}

\begin{theorem}[Birkhoff]
\(L\) is a nondistributive lattice iff \(M_5\), or \(N_5\) can be embedded into \(L\)
\end{theorem}

\begin{proof}
Let suppose that \(L\) is a nondistributive lattice and that \(L\) does not contain
a copy of \(N_5\) as a sublattice. Thus \(L\) is modular by Theorem \ref{thm3.5}.
Since the distributive laws do not hold in \(L\), there must be elements
\(a,b,c\) from \(L\) s.t. \((a\wedge b)\vee(a\wedge c)<a\wedge(b\vee c)\). Let
us define
\begin{align*}
d&=(a\wedge b)\vee(a\wedge c)\vee(b\wedge c)\\
e&=(a\vee b)\wedge(a\vee c)\wedge(b\vee c)\\
a_1&=(a\wedge e)\vee d\\
b_1&=(b\wedge e)\vee d\\
c_1&=(c\wedge e)\vee d
\end{align*}

Then \(d\le a_1,b_1,c_1\le e\). Now from
\begin{equation*}
a\wedge e=a\wedge(b\vee c)
\end{equation*}
and
\begin{align*}
a\wedge d&=\underline{a}\wedge(\underline{(a\wedge b)\vee(a\wedge c)}\vee(b\wedge c))\\
&=((a\wedge b)\vee(a\wedge c))\vee(a\wedge(b\wedge c))\tag*{by M}\\
&=(a\wedge b)\vee(a\wedge c)
\end{align*}
it follows that \(d<e\)

We now show that diagram in Figure \ref{fig:3.6} is a copy of \(M_5\) in \(L\). To
do this it suffices to show that 
\(a_1\wedge b_1=a_1\wedge c_1=b_1\wedge c_1=d\) 
and \(a_1\vee b_1=a_1\vee c_1=b_1\vee c_1=e\).


\begin{figure}
\centering
\begin{tikzpicture}
[dot/.style={circle,draw,minimum width=4pt,inner sep=1pt}]
\node[dot,label=left:$a_1$] (a) at (0,0) {};
\node[dot,label=right:$b_1$] (b) at (1,0) {};
\node[dot,label=right:$c_1$] (c) at (2,0) {};
\node[dot,label=below:$d$] (d) at (1,-1) {};
\node[dot,label=above:$e$] (e) at (1,1) {};
\path[] (e) edge (a) edge (b) edge (c)
(d) edge (a) edge (b) edge (c);
\end{tikzpicture}
\caption{}
\label{fig:3.6}
\end{figure}

\begin{align*}
a_1\wedge b_1&=((a\wedge e)\vee\underline{d})\wedge(\underline{(b\wedge e)\vee d})\\
&=((a\wedge e)\wedge((b\wedge\underline{e})\vee d))\vee d\tag*{(by M)}\\
&y\wedge z=((b\wedge e)\vee d)\wedge d=d\\
&=((a\wedge e)\wedge((b\vee d)\wedge e))\vee d\tag*{(by M)}\\
&=((a\wedge e)\wedge e\wedge(b\vee d))\vee d\\
&=((a\wedge e)\wedge(b\vee d))\vee d\\
&=(a\wedge\underline{(b\vee c)}\wedge(\underline{b}\vee(a\wedge c)))\vee d\\
&=(a\wedge(b\vee((b\vee c)\wedge(a\vee c))))\vee d\tag*{(by M)}\\
&=(\underline{a}\wedge(b\vee\underline{(a\wedge c)}))\vee d
\tag*{$a\wedge c\le b\vee c$}\\
&=(a\wedge c)\vee(b\wedge a)\vee d\tag*{(by M)}\\
&=d
\end{align*}
\end{proof}


\subsection{Complete Lattices, Equivalence Relations, and Algebraic Lattices}
\label{sec:orge617864}
\begin{definition}[]
A poset \(P\) is \textbf{complete} if for every subset \(A\) of \(P\) both \(\sup A\) and
\(\inf A\) exists in \(P\). The elements \(\sup A\) an \(\inf A\) will be
denoted by \(\bigvee A\) and \(\bigwedge A\).
\end{definition}

\begin{theorem}[]
Let \(P\) be a poset s.t. \(\bigvee A\) exists for every subset \(A\), or s.t. 
\(\bigwedge A\) exists for every subset \(A\). Then \(P\) is a complete lattice
\end{theorem}

\begin{proof}
Suppose \(\bigwedge A\) exists for every \(A\subseteq P\). Then letting \(A^u\)
be the set of upper bounds of \(A\) in \(P\), it is routine to verify that
\(\wedge A^u\) is indeed \(\vee A\).
\end{proof}

In the above theorem, the existence of \(\bigwedge\emptyset\) guarantees a
largest element in \(P\), and likewise the existence of \(\bigvee\emptyset\)
guarantees a smallest element in \(P\). (Every element is larger than
\(\emptyset\)).

\begin{definition}[]
A sublattice \(L'\) of a complete lattice \(L\) is called a \textbf{complete sublattice}
of \(L\) if for every subset \(A\) of \(L'\) the elements \(\bigvee A\) and
\(\bigwedge A\), as defined in \(L\), are actually in \(L'\)
\end{definition}
\end{document}